theories/examples/map_reduce.v
@@ -1,0 +1,454 @@
+From stdpp Require Import sorting.
+From osiris.channel Require Import proto_channel proofmode.
+From iris.heap_lang Require Import proofmode notation.
+From osiris.utils Require Import list compare spin_lock contribution.
+From osiris.examples Require Import mapper sort_elem sort_elem_client.
+From iris.algebra Require Import gmultiset.
+From Coq Require Import SetoidPermutation.
+
+(** Functional version of map reduce (aka the specification) *)
+Fixpoint group_insert {A} `{EqDecision K} (i : K) (x : A)
+    (ixss : list (K * list A)) : list (K * list A) :=
+  match ixss with
+  | [] => [(i,[x])]
+  | (j,xs) :: ixss =>
+     if decide (i = j) then (j,x::xs) :: ixss else (j,xs) :: group_insert i x ixss
+  end.
+
+Fixpoint group {A} `{EqDecision K} (ixs : list (K * A)) : list (K * list A) :=
+  match ixs with
+  | [] => []
+  | (i,x) :: ixs => group_insert i x (group ixs)
+  end.
+
+Definition map_reduce {A B C} `{EqDecision K}
+    (map : A → list (K * B)) (red : K → list B → list C) : list A → list C :=
+  mbind (curry red) ∘ group ∘ mbind map.
+
+Instance: Params (@group_insert) 5.
+Instance: Params (@group) 3.
+Instance: Params (@group) 7.
+
+(** Properties about the functional version *)
+Local Infix "≡ₚₚ" :=
+  (PermutationA (prod_relation (=) (≡ₚ))) (at level 70, no associativity) : stdpp_scope.
+Notation "(≡ₚₚ)" := (PermutationA (prod_relation (=) (≡ₚ))) (only parsing) : stdpp_scope.
+
+Section group.
+  Context {A : Type} `{EqDecision K}.
+  Implicit Types i : K.
+  Implicit Types xs : list A.
+  Implicit Types ixs : list (K * A).
+  Implicit Types ixss : list (K * list A).
+
+  Lemma elem_of_group_insert j i x ixss :
+    j ∈ (group_insert i x ixss).*1 → i = j ∨ j ∈ ixss.*1.
+  Proof.
+    induction ixss as [|[i' x'] ixss IH];
+      repeat (simplify_eq/= || case_decide); set_solver.
+  Qed.
+
+  Lemma group_insert_commute i1 i2 x1 x2 ixss :
+    group_insert i1 x1 (group_insert i2 x2 ixss) ≡ₚₚ group_insert i2 x2 (group_insert i1 x1 ixss).
+  Proof.
+    induction ixss as [|[j x] ixss IH]; repeat (simplify_eq/= || case_decide);
+      repeat constructor; done.
+ Qed.
+
+  Lemma group_insert_nodup i x ixss :
+    NoDup ixss.*1 → NoDup (group_insert i x ixss).*1.
+  Proof.
+    pose proof @elem_of_group_insert.
+    induction ixss as [|[j xs] ixss IH]; csimpl; inversion_clear 1;
+      repeat (simplify_eq/= || case_decide); repeat constructor; set_solver.
+  Qed.
+  Lemma group_nodup ixs : NoDup (group ixs).*1.
+  Proof.
+    induction ixs as [|[i x] ixs IH]; csimpl;
+      auto using group_insert_nodup, NoDup_nil_2.
+  Qed.
+
+  Lemma grouped_permutation_elem_of ixss1 ixss2 i :
+    ixss1 ≡ₚₚ ixss2 → i ∈ ixss1.*1 → i ∈ ixss2.*1.
+  Proof.
+    induction 1 as [|[i1 xs1] [i2 xs2] ixss1 ixss2 [??]|[i1 xs1] [i2 xs2] ixss|];
+      set_solver.
+  Qed.
+
+  Lemma grouped_permutation_nodup ixss1 ixss2 :
+    ixss1 ≡ₚₚ ixss2 → NoDup ixss1.*1 → NoDup ixss2.*1.
+  Proof.
+    pose proof @grouped_permutation_elem_of.
+    induction 1 as [|[i1 xs1] [i2 xs2] ixss1 ixss2 [??]|[i1 xs1] [i2 xs2] ixss|];
+      csimpl; rewrite ?NoDup_cons; try set_solver.
+  Qed.
+
+  Lemma group_insert_perm ixss1 ixss2 i x :
+    NoDup ixss1.*1 →
+    ixss1 ≡ₚₚ ixss2 → group_insert i x ixss1 ≡ₚₚ group_insert i x ixss2.
+  Proof.
+    induction 2 as [|[i1 xs1] [i2 xs2] ixss1 ixss2 [??]|[i1 xs1] [i2 xs2] ixss|];
+      repeat match goal with
+      | _ => progress (simplify_eq/= || case_decide)
+      | H : NoDup (_ :: _) |- _ => inversion_clear H
+      end; first [repeat constructor; by auto
+                 |set_solver
+                 |etrans; eauto using grouped_permutation_nodup].
+  Qed.
+
+  Global Instance group_perm : Proper ((≡ₚ) ==> (≡ₚₚ)) (@group A K _).
+  Proof.
+    induction 1; repeat (simplify_eq/= || case_decide || case_match);
+      first [by etrans|auto using group_insert_perm, group_nodup, group_insert_commute].
+  Qed.
+
+  Lemma group_fmap (i : K) xs : xs ≠ [] → group ((i,) <$> xs) ≡ₚₚ [(i, xs)].
+  Proof.
+    induction xs as [|x1 [|x2 xs] IH]; intros; simplify_eq/=; try done.
+    etrans.
+    { apply group_insert_perm, IH; auto using group_insert_nodup, group_nodup. }
+    simpl; by case_decide.
+  Qed.
+  Lemma group_insert_snoc ixss i x j ys :
+    i ≠ j →
+    group_insert i x (ixss ++ [(j, ys)]) ≡ₚₚ group_insert i x ixss ++ [(j,ys)].
+  Proof.
+    intros. induction ixss as [|[i' xs'] ixss IH];
+      repeat (simplify_eq/= || case_decide); repeat constructor; by auto.
+  Qed.
+  Lemma group_snoc ixs j ys :
+    j ∉ ixs.*1 → ys ≠ [] → group (ixs ++ ((j,) <$> ys)) ≡ₚₚ group ixs ++ [(j,ys)].
+  Proof.
+    induction ixs as [|[i x] ixs IH]; csimpl; first by auto using group_fmap.
+    rewrite ?not_elem_of_cons=> -[??]. etrans; last by apply group_insert_snoc.
+    apply group_insert_perm, IH; auto using group_nodup.
+  Qed.
+End group.
+
+Section map_reduce.
+  Context {A B C} `{EqDecision K} (map : A → list (K * B)) (red : K → list B → list C).
+  Context `{!∀ j, Proper ((≡ₚ) ==> (≡ₚ)) (red j)}.
+
+  Global Instance bind_red_perm : Proper ((≡ₚₚ) ==> (≡ₚ)) (mbind (curry red)).
+  Proof.
+    induction 1 as [|[i1 xs1] [i2 xs2] ixss1 ixss2 [??]|[i1 xs1] [i2 xs2] ixss|];
+      simplify_eq/=; try done.
+    - repeat (done || f_equiv).
+    - by rewrite !assoc_L (comm _ (red i2 xs2)).
+    - by etrans.
+  Qed.
+  Global Instance map_reduce_perm : Proper ((≡ₚ) ==> (≡ₚ)) (map_reduce map red).
+  Proof. intros xs1 xs2 Hxs. by rewrite /map_reduce /= Hxs. Qed.
+End map_reduce.
+
+(** Distributed version *)
+Definition map_reduce_service_map_loop : val :=
+  rec: "go" "n" "cmap" "csort" "xs" :=
+    if: "n" = #0 then #() else
+    if: recv "cmap" then (* send item to mapper *)
+      if: lisnil "xs" then
+        send "cmap" #false;;
+        "go" ("n" - #1) "cmap" "csort" "xs"
+      else
+        send "cmap" #true;;
+        send "cmap" (lhead "xs");;
+        "go" "n" "cmap" "csort" (ltail "xs")
+    else (* receive item from mapper *)
+      let: "zs" := recv "cmap" in
+      send_all "csort" "zs";;
+      "go" "n" "cmap" "csort" "xs".
+
+Definition map_reduce_service_recv_same_key : val :=
+  rec: "go" "csort" "i" "ys" :=
+    if: ~recv "csort" then (("i", "ys"), NONE) else
+    let: "jy" := recv "csort" in
+    let: "j" := Fst "jy" in let: "y" := Snd "jy" in
+    if: "i" = "j" then "go" "csort" "j" (lcons "y" "ys") else
+    (("i", "ys"), SOME ("j", "y")).
+
+Definition map_reduce_service_reduce_loop : val :=
+  rec: "go" "n" "csort" "cred" "acc" "zs" :=
+    if: "n" = #0 then "zs" else
+    if: recv "cred" then (* Send item to mapper *)
+      match: "acc" with
+        NONE =>
+         (* nothing left *)
+         send "cred" #false;; "go" ("n" - #1) "csort" "cred" NONE "zs"
+      | SOME "acc" =>
+         (* Read subsequent items with the same key *)
+         let: "grp" := map_reduce_service_recv_same_key "csort"
+           (Fst "acc") (lcons (Snd "acc") (lnil #())) in
+         send "cred" #true;;
+         send "cred" (Fst "grp");;
+         "go" "n" "csort" "cred" (Snd "grp") "zs"
+      end
+    else (* receive item from mapper *)
+      let: "zs'" := recv "cred" in
+      "go" "n" "csort" "cred" "acc" (lapp "zs'" "zs").
+
+Definition cmpZfst : val := λ: "x" "y", Fst "x" ≤ Fst "y".
+
+Definition map_reduce_service : val := λ: "n" "map" "red" "xs",
+  let: "lmap" := new_lock #() in
+  let: "cmap" := start_chan (λ: "c", start_mappers "n" "map" "lmap" "c") in
+  let: "csort" := start_chan (λ: "c", sort_elem_service cmpZfst "c") in
+  map_reduce_service_map_loop "n" "cmap" "csort" "xs";;
+  send "csort" #stop;;
+  let: "lred" := new_lock #() in
+  let: "cred" := start_chan (λ: "c", start_mappers "n" "red" "lred" "c") in
+  (* Fetch the first sorted element, which we need in the loop *)
+  if: ~recv "csort" then lnil #() else (* Handle the empty case *)
+  let: "jy" := recv "csort" in
+  map_reduce_service_reduce_loop "n" "csort" "cred" (SOME "jy") (lnil #()).
+
+(** Correctness proofs of the distributed version *)
+Class map_reduceG Σ A B `{Countable A, Countable B} := {
+  map_reduce_mapG :> mapperG Σ A;
+  map_reduce_reduceG :> mapperG Σ (Z * list B);
+}.
+
+Section mapper.
+  Context `{Countable A, Countable B} {C : Type}.
+  Context `{!heapG Σ, !proto_chanG Σ, !lockG Σ, !map_reduceG Σ A B} (N : namespace).
+  Context (IA : A → val → iProp Σ) (IB : Z → B → val → iProp Σ) (IC : C → val → iProp Σ).
+  Context (map : A → list (Z * B)) (red : Z → list B → list C).
+  Context `{!∀ j, Proper ((≡ₚ) ==> (≡ₚ)) (red j)}.
+  Local Open Scope nat_scope.
+
+  Definition IZB (iy : Z * B) (w : val) : iProp Σ :=
+    (∃ w', ⌜ w = (#iy.1, w')%V ⌝ ∧ IB iy.1 iy.2 w')%I.
+  Definition IZBs (iys : Z * list B) (w : val) : iProp Σ :=
+    (∃ ws, ⌜ w = (#iys.1, llist ws)%V ⌝ ∧ [∗ list] y;w'∈iys.2;ws, IB iys.1 y w')%I.
+  Definition RZB : relation (Z * B) := prod_relation (≤)%Z (λ _ _ : B, True).
+
+  Instance RZB_dec : RelDecision RZB.
+  Proof. solve_decision. Qed.
+  Instance RZB_total : Total RZB.
+  Proof. intros [i1 y1] [i2 y2]. destruct (total (≤)%Z i1 i2); [left|right]; done. Qed.
+  Instance RZB_trans : Transitive RZB.
+  Proof. by apply (prod_relation_trans _). Qed.
+  Lemma RZB_cmp_spec : cmp_spec IZB RZB cmpZfst.
+  Proof.
+    iIntros ([i1 y1] [i2 y2] v1 v2) "!>"; iIntros (Φ) "[HI1 HI2] HΦ".
+    iDestruct "HI1" as (w1 ->) "HI1". iDestruct "HI2" as (w2 ->) "HI2 /=".
+    wp_lam; wp_pures. iSpecialize ("HΦ" with "[HI1 HI2]").
+    { iSplitL "HI1"; rewrite /IZB /=; eauto with iFrame. }
+    repeat case_bool_decide=> //; unfold RZB, prod_relation in *; naive_solver.
+  Qed.
+
+  Lemma map_reduce_service_map_loop_spec (n : nat) cmap csort vs xs X ys :
+    (n = 0 → X = ∅ ∧ xs = []) →
+    {{{
+      cmap ↣ mapper_protocol IA IZB map n (X : gmultiset A) @ N ∗
+      csort ↣ sort_elem_head_protocol IZB RZB ys @ N ∗
+      ([∗ list] x;v ∈ xs;vs, IA x v)
+    }}}
+      map_reduce_service_map_loop #n cmap csort (llist vs)
+    {{{ ys', RET #();
+      ⌜ys' ≡ₚ (xs ++ elements X) ≫= map⌝ ∗
+      csort ↣ sort_elem_head_protocol IZB RZB (ys ++ ys') @ N
+    }}}.
+  Proof.
+    iIntros (Hn Φ) "(Hcmap & Hcsort & HIA) HΦ".
+    iLöb as "IH" forall (n vs xs X ys Hn Φ); wp_rec; wp_pures; simpl.
+    case_bool_decide; wp_pures; simplify_eq/=.
+    { destruct Hn as [-> ->]; first lia.
+      iApply ("HΦ" $! []). rewrite right_id_L. auto. }
+    destruct n as [|n]=> //=. wp_branch as %?|%_; wp_pures.
+    - wp_apply (lisnil_spec with "[//]"); iIntros (_).
+      destruct vs as [|v vs], xs as [|x xs]; csimpl; try done; wp_pures.
+      + wp_select. wp_pures. rewrite Nat2Z.inj_succ Z.sub_1_r Z.pred_succ.
+        iApply ("IH" $! _ _ [] with "[%] Hcmap Hcsort [//] HΦ"); naive_solver.
+      + iDestruct "HIA" as "[HIAx HIA]". wp_select.
+        wp_apply (lhead_spec with "[//]"); iIntros (_).
+        wp_send with "[$HIAx]".
+        wp_apply (ltail_spec with "[//]"); iIntros (_).
+        wp_apply ("IH" with "[%] Hcmap Hcsort HIA"); first done.
+        iIntros (ys').
+        rewrite gmultiset_elements_disj_union gmultiset_elements_singleton.
+        rewrite assoc_L -(comm _ [x]). iApply "HΦ".
+    - wp_recv (x w) as (Hx) "HIBfx".
+      rewrite -(right_id END%proto _ (sort_elem_head_protocol _ _ _)).
+      wp_apply (send_all_spec with "[$Hcsort $HIBfx]"); iIntros "Hcsort".
+      rewrite right_id.
+      wp_apply ("IH" with "[] Hcmap Hcsort HIA"); first done.
+      iIntros (ys'). iDestruct 1 as (Hys) "Hcsort"; simplify_eq/=.
+      rewrite -assoc_L. iApply ("HΦ" $! (map x ++ ys') with "[$Hcsort]").
+      iPureIntro. rewrite (gmultiset_disj_union_difference {[ x ]} X)
+        -?gmultiset_elem_of_singleton_subseteq //.
+      rewrite (comm disj_union) gmultiset_elements_disj_union.
+      by rewrite gmultiset_elements_singleton assoc_L bind_app -Hys /= right_id_L comm.
+  Qed.
+
+  Lemma map_reduce_service_recv_same_key_spec csort iys iys_sorted i ys ws :
+    let acc := from_option (λ '(i,y,w), [(i,y)]) [] in
+    let accv := from_option (λ '(i,y,w), SOMEV (#(i:Z),w)) NONEV in
+    ys ≠ [] →
+    Sorted RZB (iys_sorted ++ ((i,) <$> ys)) →
+    i ∉ iys_sorted.*1 →
+    {{{
+      csort ↣ sort_elem_tail_protocol IZB RZB iys (iys_sorted ++ ((i,) <$> ys)) @ N ∗
+      [∗ list] y;w ∈ ys;ws, IB i y w
+    }}}
+      map_reduce_service_recv_same_key csort #i (llist (reverse ws))
+    {{{ ys' ws' miy, RET ((#i,llist (reverse ws')),accv miy);
+      ⌜ Sorted RZB ((iys_sorted ++ ((i,) <$> ys ++ ys')) ++ acc miy) ⌝ ∗
+      ⌜ from_option (λ '(j,_,_), i ≠ j ∧ j ∉ iys_sorted.*1)
+                    (iys_sorted ++ ((i,) <$> ys ++ ys') ≡ₚ iys) miy ⌝ ∗
+      csort ↣ from_option (λ _, sort_elem_tail_protocol IZB RZB iys
+        ((iys_sorted ++ ((i,) <$> ys ++ ys')) ++ acc miy)) END%proto miy @ N ∗
+      ([∗ list] y;w ∈ ys ++ ys';ws', IB i y w) ∗
+      from_option (λ '(i,y,w), IB i y w) True miy
+    }}}.
+  Proof.
+    iIntros (acc accv Hys Hsort Hi Φ) "[Hcsort HIB] HΦ".
+    iLöb as "IH" forall (ys ws Hys Hsort Hi Φ); wp_rec; wp_pures; simpl.
+    wp_branch as %_|%Hperm; last first; wp_pures.
+    { iApply ("HΦ" $! [] _ None with "[$Hcsort HIB]"); simpl.
+     iEval (rewrite !right_id_L); auto. }
+    wp_recv ([j y] ?) as (Htl w ->) "HIBy /=". wp_pures. rewrite -assoc_L.
+    case_bool_decide as Hij; simplify_eq/=; wp_pures.
+    - wp_apply (lcons_spec with "[//]"); iIntros (_).
+      rewrite -reverse_snoc. wp_apply ("IH" $! (ys ++ [y])
+        with "[%] [%] [//] [Hcsort] [HIB HIBy] [HΦ]"); try iClear "IH".
+      + intros ?; discriminate_list.
+      + rewrite fmap_app /= assoc_L. by apply Sorted_snoc.
+      + by rewrite fmap_app /= assoc_L.
+      + iApply (big_sepL2_app with "HIB"). by iFrame.
+      + iIntros "!>" (ys' ws' miy). rewrite -!(assoc_L _ ys) /=.
+        iApply ("HΦ" $! (y :: ys')).
+    - iApply ("HΦ" $! [] _ (Some (j,y,w))).
+      rewrite /= !right_id_L assoc_L. iFrame. iPureIntro; split.
+      { by apply Sorted_snoc. }
+      split; first congruence.
+      intros [[j' y'] [-> Hj]]%elem_of_list_fmap.
+      destruct Hij; do 2 f_equal.
+      destruct ys as [|y'' ys _] using rev_ind; first done.
+      move: Htl. rewrite fmap_app assoc_L /=.
+      inversion 1 as [|?? [? _]]; discriminate_list || simplify_list_eq.
+      assert (RZB (j',y') (i,y'')) as [??]; last (simpl in *; lia).
+      apply (Sorted_StronglySorted _) in Hsort.
+      eapply elem_of_StronglySorted_app; set_solver.
+  Qed.
+
+  Lemma mapper_service_loop_spec (n : nat) iys iys_sorted miy zs ws Y csort cred :
+    let acc := from_option (λ '(i,y,w), [(i,y)]) [] in
+    let accv := from_option (λ '(i,y,w), SOMEV (#(i:Z),w)) NONEV in
+    (n = 0 → miy = None ∧ Y = ∅) →
+    from_option (λ '(i,_,_), i ∉ iys_sorted.*1) (iys_sorted ≡ₚ iys) miy →
+    Sorted RZB (iys_sorted ++ acc miy) →
+    {{{
+      csort ↣ from_option (λ _, sort_elem_tail_protocol IZB RZB iys
+        (iys_sorted ++ acc miy)) END%proto miy @ N ∗
+      cred ↣ mapper_protocol IZBs IC (curry red) n (Y : gmultiset (Z * list B)) @ N ∗
+      from_option (λ '(i,y,w), IB i y w) True miy ∗
+      ([∗ list] z;w ∈ zs;ws, IC z w)
+    }}}
+      map_reduce_service_reduce_loop #n csort cred (accv miy) (llist ws)
+    {{{ zs' ws', RET (llist ws');
+       ⌜ (group iys_sorted ≫= curry red) ++ zs' ≡ₚ (group iys ++ elements Y) ≫= curry red ⌝ ∗
+       [∗ list] z;w ∈ zs' ++ zs;ws', IC z w
+    }}}.
+  Proof.
+    iIntros (acc accv Hn Hmiy Hsort Φ) "(Hcsort & Hcred & HIB & HIC) HΦ".
+    iLöb as "IH" forall (n iys_sorted miy zs ws Y Hn Hmiy Hsort Φ); wp_rec; wp_pures; simpl.
+    case_bool_decide; wp_pures; simplify_eq/=.
+    { destruct Hn as [-> ->]; first lia.
+      iApply ("HΦ" $! [] with "[$HIC]"); iPureIntro; simpl.
+      by rewrite gmultiset_elements_empty !right_id_L Hmiy. }
+    destruct n as [|n]=> //=. wp_branch as %?|%_; wp_pures.
+    - destruct miy as [[[i y] w]|]; simplify_eq/=; wp_pures; last first.
+      + wp_select. wp_pures. rewrite Nat2Z.inj_succ Z.sub_1_r Z.pred_succ.
+        iApply ("IH" $! _ _ None
+          with "[%] [%] [%] Hcsort Hcred [] HIC HΦ"); naive_solver.
+      + wp_apply (lnil_spec with "[//]"); iIntros (_).
+        wp_apply (lcons_spec with "[//]"); iIntros (_).
+        wp_apply (map_reduce_service_recv_same_key_spec _ _ _ _ [_] [_]
+          with "[$Hcsort HIB]"); try done.
+        { simpl; iFrame. }
+        iIntros (ys' ws'' miy).
+        iDestruct 1 as (? Hmiy') "(Hcsort & HIB & HIC')"; csimpl.
+        wp_select; wp_pures. wp_send ((i, reverse (y :: ys'))) with "[HIB]".
+        { iExists (reverse ws''); rewrite /= big_sepL2_reverse; auto. }
+        wp_pures. iApply ("IH" $! _ (_ ++ _) miy
+          with "[%] [%] [//] Hcsort Hcred HIC' HIC"); first done.
+        { destruct miy as [[[i' y'] w']|]; set_solver +Hmiy'. }
+        iIntros "!>" (zs' ws'''). iDestruct 1 as (Hperm) "HIC".
+        iApply ("HΦ" with "[$HIC]"); iPureIntro; move: Hperm.
+        rewrite gmultiset_elements_disj_union gmultiset_elements_singleton.
+        rewrite group_snoc // reverse_Permutation.
+        rewrite !bind_app /= right_id_L -!assoc_L -(comm _ zs') !assoc_L.
+        apply (inj (++ _)).
+    - wp_recv ([i ys] ws') as (Hy) "HICi".
+      wp_apply (lapp_spec with "[//]"); iIntros (_).
+      wp_apply ("IH" $! _ _ _ (_ ++ _)
+        with "[ ] [//] [//] Hcsort Hcred HIB [HIC HICi]"); first done.
+      { simpl; iFrame. }
+      iIntros (zs' ws''); iDestruct 1 as (Hzs) "HIC"; simplify_eq/=.
+      iApply ("HΦ" $! (zs' ++ red i ys)). iSplit; last by rewrite -assoc_L.
+      iPureIntro. rewrite (gmultiset_disj_union_difference {[ i,ys ]} Y)
+        -?gmultiset_elem_of_singleton_subseteq //.
+      rewrite (comm disj_union) gmultiset_elements_disj_union.
+      rewrite gmultiset_elements_singleton assoc_L Hzs !bind_app /=.
+      by rewrite right_id_L !assoc_L.
+  Qed.
+
+  Definition map_spec (vmap : val) : iProp Σ := (∀ x v,
+    {{{ IA x v }}}
+      vmap v
+    {{{ ws, RET (llist ws); [∗ list] iy;w ∈ map x;ws, IZB iy w }}})%I.
+  Definition red_spec (vred : val) : iProp Σ := (∀ i ys vs,
+    {{{ [∗ list] y;v ∈ ys;vs, IB i y v }}}
+      vred (#i, llist vs)%V
+    {{{ ws, RET (llist ws); [∗ list] z;w ∈ red i ys;ws, IC z w }}})%I.
+
+  Lemma map_reduce_service_spec (n : nat) vmap vred vs xs :
+    0 < n →
+    map_spec vmap -∗
+    red_spec vred -∗
+    {{{ [∗ list] x;v ∈ xs;vs, IA x v }}}
+      map_reduce_service #n vmap vred (llist vs)
+    {{{ zs ws, RET (llist ws);
+      ⌜zs ≡ₚ map_reduce map red xs⌝ ∗ [∗ list] z;w ∈ zs;ws, IC z w
+    }}}.
+  Proof.
+    iIntros (?) "#Hmap #Hred !>"; iIntros (Φ) "HI HΦ". wp_lam; wp_pures.
+    wp_apply (new_lock_spec N with "[//]"); iIntros (lkmap) "[Hu Hlk]".
+    wp_apply (start_chan_proto_spec N (mapper_protocol IA IZB map n ∅)
+      with "[Hu Hlk]"); try iNext; iIntros (cmap) "Hcmap".
+    { wp_lam.
+      iMod (contribution_init_pow (A:=gmultisetUR A) n) as (γ) "[Hs Hγs]".
+      iMod ("Hlk" $! (mapper_lock_inv N IA IZB map γ cmap) with "[Hcmap Hs]") as "#Hlk".
+      { iExists n, ∅. iFrame. }
+      wp_apply (start_mappers_spec with "Hmap [$Hlk $Hu $Hγs]"); auto. }
+    wp_apply (start_chan_proto_spec N (sort_elem_protocol IZB RZB <++> END)%proto);
+      iIntros (csort) "Hcsort".
+    { wp_apply (sort_elem_service_spec N with "[] Hcsort"); last by auto.
+      iApply RZB_cmp_spec. }
+    rewrite right_id.
+    wp_apply (map_reduce_service_map_loop_spec with "[$Hcmap $Hcsort $HI]"); first lia.
+    iIntros (iys). rewrite gmultiset_elements_empty right_id_L.
+    iDestruct 1 as (Hiys) "Hcsort /=". wp_select; simpl.
+    wp_apply (new_lock_spec N with "[//]"); iIntros (lkred) "[Hu Hlk]".
+    wp_apply (start_chan_proto_spec N (mapper_protocol IZBs IC (curry red) n ∅)
+      with "[Hu Hlk]"); try iNext; iIntros (cred) "Hcred".
+    { wp_lam.
+      iMod (contribution_init_pow (A:=gmultisetUR (Z * list B)) n) as (γ) "[Hs Hγs]".
+      iMod ("Hlk" $! (mapper_lock_inv N IZBs IC (curry red) γ cred)
+        with "[Hcred Hs]") as "#Hlk".
+      { iExists n, ∅. iFrame. }
+      wp_apply (start_mappers_spec with "[Hred] [$Hlk $Hu $Hγs]"); last by auto.
+      iIntros ([i ys] v) "!>"; iIntros (Ψ); iDestruct 1 as (ws ->) "HIB".
+      iIntros "HΦ /=". iApply ("Hred" with "HIB HΦ"). }
+    wp_branch as %_|%Hnil; last first.
+    { wp_pures. wp_apply (lnil_spec with "[//]"); iIntros (_).
+      iApply ("HΦ" $! []); simpl. iSplit; [iPureIntro|done].
+      by rewrite /map_reduce /= -Hiys -Hnil. }
+    wp_recv ([i y] ?) as (_ w ->) "HIB /="; wp_pures.
+    wp_apply (lnil_spec with "[//]"); iIntros (_).
+    wp_apply (mapper_service_loop_spec _ _ [] (Some (i, y, w)) [] []
+      with "[$Hcsort $Hcred $HIB]"); simpl; auto; [lia|set_solver|].
+    iIntros (zs ws). rewrite /= gmultiset_elements_empty !right_id.
+    iDestruct 1 as (Hzs) "HIC". iApply ("HΦ" with "[$HIC]"). by rewrite Hzs Hiys.
+  Qed.
+End mapper.
